add more implementation

StackLean/Basic.lean
@@ -11,16 +11,22 @@ inductive Slot where
   | Var : Nat → Slot
   | Lit : Word → Slot
   | Junk : Slot
-  deriving BEq, Hashable, DecidableEq
+  deriving BEq, Hashable, Hashable, DecidableEq
 
 abbrev Stack := List Slot
 
 structure Target where
   args : Stack
+  -- TODO: make this a Set
   tail : Multiset Slot
 
+inductive Ty where
+  | Int : Ty
+  | Bool : Ty
+
 inductive Op where
-  | Swap     : Fin 16 → Op
+  -- swap0 is a noop, the others match the evm
+  | Swap     : Fin 17 → Op
   | Dup      : Fin 16 → Op
   | Pop      : Op
   | Push     : Word → Op
@@ -35,7 +41,7 @@ def Stack.apply (stack : Stack) : Op → Except Err Stack
       if h : idx < stack.length
       then
         let s := stack.set 0 stack[idx]
-        return s.set idx stack[0]
+        return s.set (idx) stack[0]
       else throw .StackTooShallow
   | .Dup idx =>
       if h : idx < stack.length
@@ -51,26 +57,120 @@ def Stack.apply (stack : Stack) : Op → Except Err Stack
       then return stack.set idx .Junk
       else throw .StackTooShallow
 
-theorem apply_swap_inv (stack : Stack) (idx : Fin 16) (h : idx < stack.length) :
+-- apply theorems --
+
+-- applying swap at the same idx twice is a noop
+theorem apply_swap_inv (stack : Stack) (idx : Fin 17) (h : idx < stack.length) :
   stack.apply (.Swap idx) >>= (·.apply (.Swap idx)) = .ok stack := by
+    simp_all [Stack.apply, Bind.bind, Except.bind, pure, Except.pure, List.length_set]
+    ext i
+    simp [List.getElem_set]
+    split_ifs
+    · simp_all
+    · simp_all only [List.getElem?_set]
+      split_ifs <;> simp_all
+
+-- swap does not change the length of the stack
+theorem apply_swap_length (stack : Stack) (idx : Fin 17) (h : idx < stack.length) :
+  List.length <$> stack.apply (.Swap idx) = .ok stack.length := by
+    simp_all [Stack.apply, pure, Except.pure, List.length_set]
+
+-- swap switches the elem at idx with the elem at 0
+theorem apply_swap_positions_switched (stack : Stack) (idx : Fin 17) (h : idx < stack.length) :
+  ∃ (s' : Stack), stack.apply (.Swap idx) = .ok s' ∧ s'[0]? = some stack[idx] ∧ s'[idx]? = some stack[0] := by
+  simp_all [Stack.apply, pure, Except.pure, List.length_set, List.getElem?_set]
+  split_ifs <;> simp_all
+
+-- dup grows stack size by 1
+theorem apply_dup_grows_stack (stack : Stack) (idx : Fin 16) (h : idx < stack.length) :
+  (stack.apply (.Dup idx) >>= (pure $ ·.length)) = .ok (stack.length + 1) := by
+    simp_all [Stack.apply, Bind.bind, Except.bind, pure, Except.pure]
+
+-- the stack head is the same as the element at idx after applying (dup idx)
+theorem apply_dup_stack_top_eq_idx (stack : Stack) (idx : Fin 16) (h : idx < stack.length) :
+  (stack.apply (.Dup idx) >>= (pure $ ·[0]?)) = .ok (stack[idx]?) := by
+    simp_all [Stack.apply, Bind.bind, Except.bind, pure, Except.pure]
+
+-- the tail of the new stack is the same as the starting stack after applying (dup idx)
+theorem apply_dup_stack_tail_eq_prev (stack : Stack) (idx : Fin 16) (h : idx < stack.length) :
+  (stack.apply (.Dup idx) >>= (pure $ ·.tail)) = .ok (stack) := by
+    simp_all [Stack.apply, Bind.bind, Except.bind, pure, Except.pure]
+
+-- the result of applying pop is the same as the tail of the input stack
+theorem apply_pop_eq_prev_stack_tail (stack : Stack) (h : stack.length > 0) :
+  stack.apply .Pop = .ok (stack.tail) := by
     simp_all [Stack.apply, pure, Except.pure]
-    sorry
 
+-- TODO: push / markjunk theorems
 
+-- shuffle --
 
---def shuffle (stack : Stack) (target : Target) : Except Err Stack := do
-  --let (head, tail) := stack.splitAt target.args.length
-  ---- check if the current head matches the target head
-  --if head == target.args then
-    ---- check if any of the args are also required in the tail and not there yet
-    --let missing := (target.tail - (Multiset.ofList tail)).toFinset
-    --for slot in missing do
-      --match head.findIdx? (· == slot) with
-      --| .none => continue
-      --| .some idx =>
-        --if h : idx < 16 then
-          --return path ++ [Op.Dup ⟨idx, h⟩]
-        --else
-          --throw "Can't dup past 16..."
-    --return path
-  --return path
+-- TODO: using Multiset is nice but idk how to make it computable
+-- TODO: target can only be reached from stack if the variable set of target ⊆ the variable set of stack
+noncomputable def shuffle (stack : Stack) (target : Target) : Except Err Stack := do
+  if h_stack_empty : stack = [] then
+    throw .StackTooShallow
+  else
+
+    let head := stack.take target.args.length
+    let tail := stack.drop target.args.length
+
+    -- check if the current head matches the target head
+    if hargs : head = target.args then
+      -- check if any of the args are also required in the tail and not there yet
+      -- TODO: I'm probably handling junk wrong here
+      let missing := (target.tail - (Multiset.ofList tail)).toFinset.toList
+      for slot in missing do
+        match head.findIdx? (· == slot) with
+        | .none => continue
+        -- dup if that is the case (or dup deep slot if required)
+        -- TODO: what does dup deep slot if required mean??
+        | .some idx =>
+          if h : idx < 16 then
+            let s' ← stack.apply (.Dup ⟨idx, h⟩)
+            -- TODO: recurse
+            return s'
+          else
+            throw .StackTooDeep
+      -- otherwise return, we are done
+      return stack
+
+    else
+
+      -- invariant: the args region is wrong
+      have h_wrong : head ≠ target.args := by simp_all
+      -- invariant: the args region is non empty
+      have h_non_empty : head ≠ [] := by
+        by_contra h_empty
+        have h_args_empty : target.args = []:= by simp_all [head]
+        simp_all
+
+      -- helper lemma for safe indexing proofs
+      have : 0 < stack.length := by exact List.length_pos_iff.mpr h_stack_empty
+
+      let top := stack[0]
+      let top_is_surplus_in_args := top ∈ (Multiset.ofList head - target.args)
+      let top_is_surplus_in_tail := top ∈ (Multiset.ofList tail - target.tail)
+
+      -- if the top can be popped (args and tail have enough of it without it, it’s not junk)
+      if h_top_is_surplus : top_is_surplus_in_args ∧ top_is_surplus_in_tail ∧ top ≠ .Junk then
+        -- pop it
+        let s' ← stack.apply .Pop
+        -- TODO: recurse
+        return s'
+      else
+
+        -- invariant: the top is either required in args or in tail or is junk
+        -- TODO
+
+        -- if the top is junk and popping it fixes one or more positions in args
+        if h_popping_junk_fixes_args : top = .Junk ∧ True then
+          -- pop it
+          let s' ← stack.apply .Pop
+          -- TODO: recurse
+          return s'
+
+        return stack
+
+theorem shuffle_correct : ∀ (stack : Stack) (target : Target),
+  ∃ (res : Stack), .ok res = shuffle stack target ∧ res
